Implement Model.PNE modulo one admit

src/Model.PNE.fsti
@@ -80,14 +80,14 @@ type entry (#j:id) (u:info j) =
     c:pne_cipher l ->
     entry u
 
-val pne_state : (#j:id) -> (u:info j) -> Type0
+val pne_state : (#j:id) -> (u:info j) -> Type u#1
 
-val table : (#j:id) -> (#u:info j) -> (st:pne_state u) -> (h:mem) -> GTot (Seq.seq (entry u))
+val table : (#j:safe_id) -> (#u:info j) -> (st:pne_state u) -> (h:mem) -> GTot (Seq.seq (entry u))
 
 // Header protection key
 val key: #j:unsafe_id -> #u:info j -> st:pne_state u -> h:mem -> GTot (lbytes (Spec.Agile.Cipher.key_length u.calg))
 
-val footprint : #j:id -> #u:info j -> st:pne_state u -> B.loc
+val footprint : #j:id -> #u:info j -> st:pne_state u -> GTot B.loc
 
 val invariant: #j:id -> #u:info j -> st:pne_state u -> mem -> Type0
 
@@ -103,6 +103,7 @@ val frame_table: #j:safe_id -> #u:info j -> st:pne_state u ->
   r:B.loc -> h0:mem -> h1:mem ->
   Lemma
     (requires
+      invariant st h0 /\
       B.modifies r h0 h1 /\
       r `B.loc_disjoint` (footprint st))
     (ensures table st h1 == table st h0)
@@ -115,30 +116,30 @@ let pne_bits_eq #l (x y: pne_cipher l) =
 let sample_filter (#j:id) (u:info j) (s:sample) (e:entry u) : bool =
   Entry?.s e = s
 
-let entry_for_sample (#j:id) (#u:info j) (s:sample) (st:pne_state u) (h:mem) :
+let entry_for_sample (#j:safe_id) (#u:info j) (s:sample) (st:pne_state u) (h:mem) :
   GTot (option (entry u)) =
   Seq.find_l (sample_filter u s) (table st h)
 
 /// XXX unused
-let contains_sample (#j:id) (#u:info j) (s:sample) (st:pne_state u) (h:mem) :
+let contains_sample (#j:safe_id) (#u:info j) (s:sample) (st:pne_state u) (h:mem) :
   GTot bool =
   Some? (entry_for_sample s st h)
 
-let fresh_sample (#j:id) (#u:info j) (s:sample) (st:pne_state u) (h:mem) :
+let fresh_sample (#j:safe_id) (#u:info j) (s:sample) (st:pne_state u) (h:mem) :
   GTot bool =
   None? (entry_for_sample s st h)
 
 // Finding the entry for a given cipher. Insofar as I understand, the table
 // keeps a map from plain to cipher (i.e. cipher truncated to the right length,
 // or "clipped"). XXX this seems to be unused.
-let sample_cipher_filter (j:id) (u:info j) (s:sample) (#l:pne_plain_length) (c:pne_cipher l) (e:entry u) : bool =
+let sample_cipher_filter (j:safe_id) (u:info j) (s:sample) (#l:pne_plain_length) (c:pne_cipher l) (e:entry u) : bool =
   Entry?.s e = s && Entry?.l e = l && Entry?.c e `pne_bits_eq` c
 
-let entry_for_sample_cipher (#j:id) (#u:info j) (s:sample) (#l:pne_plain_length) (c:pne_cipher l) (st:pne_state u) (h:mem) :
+let entry_for_sample_cipher (#j:safe_id) (#u:info j) (s:sample) (#l:pne_plain_length) (c:pne_cipher l) (st:pne_state u) (h:mem) :
   GTot (option (entry u)) =
   Seq.find_l (sample_cipher_filter j u s #l c) (table st h)
 
-let contains_sample_cipher (#j:id) (#u:info j) (s:sample) (#l:pne_plain_length) (c:pne_cipher l) (st:pne_state u) (h:mem) :
+let contains_sample_cipher (#j:safe_id) (#u:info j) (s:sample) (#l:pne_plain_length) (c:pne_cipher l) (st:pne_state u) (h:mem) :
   GTot bool =
   Some? (entry_for_sample_cipher s #l c st h)
 
@@ -147,14 +148,14 @@ let contains_sample_cipher (#j:id) (#u:info j) (s:sample) (#l:pne_plain_length) 
 // instead is define a successful table lookup is a match on i) the protected
 // bits, ii) the sample and iii) the truncation of the cipher. XXX this seems to
 // be unused as well.
-let sample_cipherpad_filter (#j:id) (#u:info j) (s:sample) (cp:pne_cipherpad) (e:entry u) : bool =
+let sample_cipherpad_filter (#j:safe_id) (#u:info j) (s:sample) (cp:pne_cipherpad) (e:entry u) : bool =
   Entry?.s e = s && clip_cipherpad cp (Entry?.l e) `pne_bits_eq` Entry?.c e
 
-let entry_for_sample_cipherpad (#j:id) (#u:info j) (s:sample) (cp:pne_cipherpad) (st:pne_state u) (h:mem) :
+let entry_for_sample_cipherpad (#j:safe_id) (#u:info j) (s:sample) (cp:pne_cipherpad) (st:pne_state u) (h:mem) :
   GTot (option (entry u)) =
   Seq.find_l (sample_cipherpad_filter s cp) (table st h)
 
-let contains_sample_cipherpad (#j:id) (#u:info j) (s:sample) (cp:pne_cipherpad) (st:pne_state u) (h:mem) :
+let contains_sample_cipherpad (#j:safe_id) (#u:info j) (s:sample) (cp:pne_cipherpad) (st:pne_state u) (h:mem) :
   GTot bool =
   Some? (entry_for_sample_cipherpad s cp st h)
 
@@ -169,7 +170,34 @@ val create (j:id) (u:info j) : ST (pne_state u)
     B.fresh_loc (footprint st) h0 h1 /\
     B.(loc_includes (loc_pne_region ()) (footprint st)) /\
 
-    (I.ideal_PRF && I.is_pne_honest j ==> table st h1 == Seq.empty))
+    (is_safe j ==> table st h1 == Seq.empty))
+
+let encrypt_spec (a: Spec.cipher_alg)
+  (l: pne_plain_length)
+  (pn: lbytes l)
+  (bits: protected_bits)
+  (s: sample)
+  (k: Spec.key a)
+  (pn_length: nat { 0 <= pn_length /\ pn_length <= 3 /\ l >= pn_length + 1}):
+  pne_cipher l
+=
+  let open QUIC.Spec.Lemmas in
+  // We need the packet number length in order to know where to find the mask in the cipher block.
+  let mask = QUIC.Spec.block_of_sample a k s in
+  let pnmask = and_inplace (Seq.slice mask 1 (pn_length + 2)) (QUIC.Spec.pn_sizemask_naive pn_length) 0 in
+  // Classify, because HACL* specs require secret integers.
+  let pnmask = Seq.init (Seq.length pnmask) (fun i -> Lib.IntTypes.u8 (UInt8.v (Seq.index pnmask i))) in
+  assert (Seq.length pnmask == pn_length + 1);
+  // We now have enough to build the encrypted pn. Note that because our
+  // input is a sliced packet number, we don't mask at an offset like
+  // header_encrypt does.
+  let encrypted_pn = pointwise_op (Lib.IntTypes.(logxor #U8 #SEC)) pn pnmask 0 in
+  // Now on to bit protection. Since we receive as input only the protected
+  // bits, there is a proof obligation for a caller, to show that get_bf
+  // (header.[0] `xor` mask.[0]) == get_bf header.[0] `xor` get_bf mask.[0]
+  let mask_bits: protected_bits = LowParse.BitFields.get_bitfield (UInt8.v (Seq.index mask 0)) 0 5 in
+  let protected_bits = mask_bits `FStar.UInt.logxor` bits in
+  encrypted_pn, protected_bits
 
 val encrypt :
   (#j:id) ->
@@ -183,42 +211,59 @@ val encrypt :
   (pn_length: nat { 0 <= pn_length /\ pn_length <= 3 }) ->
   ST (pne_cipher l)
   (requires fun h0 ->
+    invariant st h0 /\
     l >= pn_length + 1 /\
-    fresh_sample s st h0)
+    // JP: cannot talk about freshness because it requires talking about the
+    // table which is only available for safe id's
+    (is_safe j ==> fresh_sample s st h0))
   (ensures fun h0 c h1 ->
     B.modifies (footprint st) h0 h1 /\ (
     if is_safe j then
       table st h1 == Seq.snoc (table st h0) (Entry s #l n c)
     else
-      let open QUIC.Spec.Lemmas in
       // Our input is: plain packet number, plain bits to be protected
       let pn, bits = PNEPlainPkg?.as_bytes u.plain j l n in
+      let k = key st h0 in
       // We output an encrypted packet number and protected bits
-      let return_pn, return_bits = c in
-      // We need the packet number length in order to know where to find the mask in the cipher block.
-      let mask = QUIC.Spec.block_of_sample u.calg (key st h0) s in
-      let pnmask = and_inplace (Seq.slice mask 1 (pn_length + 2)) (QUIC.Spec.pn_sizemask_naive pn_length) 0 in
-      // Classify, because HACL* specs require secret integers.
-      let pnmask = Seq.init (Seq.length pnmask) (fun i -> Lib.IntTypes.u8 (UInt8.v (Seq.index pnmask i))) in
-      // We now have enough to build the encrypted pn. Note that because our
-      // input is a sliced packet number, we don't mask at an offset like
-      // header_encrypt does.
-      let encrypted_pn = pointwise_op (Lib.IntTypes.(logxor #U8 #SEC)) pn pnmask 0 in
-      // Now on to bit protection. Since we receive as input only the protected
-      // bits, there is a proof obligation for a caller, to show that get_bf
-      // (header.[0] `xor` mask.[0]) == get_bf header.[0] `xor` get_bf mask.[0]
-      let mask_bits: protected_bits = LowParse.BitFields.get_bitfield (UInt8.v (Seq.index mask 0)) 0 5 in
-      let protected_bits = mask_bits `FStar.UInt.logxor` bits in
-      return_pn == encrypted_pn /\ return_bits == protected_bits))
+      c == encrypt_spec u.calg l pn bits s k pn_length))
 
-val decrypt :
+let decrypt_spec
+  (#j:unsafe_id)
+  (#u:info j)
+  (a: Spec.cipher_alg)
+  (padded_cipher: lbytes 5)
+  (bits: protected_bits)
+  (k: Spec.key a)
+  (s: sample):
+  (l:pne_plain_length & pne_plain u l)
+=
+  // This mimics the specification of header_decrypt_aux starting after:
+  // let sample = ...
+  let mask = QUIC.Spec.block_of_sample a k s in
+  // Decrypting protected bits
+  let mask_bits: protected_bits = LowParse.BitFields.get_bitfield (UInt8.v (Seq.index mask 0)) 0 5 in
+  let bits = mask_bits `FStar.UInt.logxor` bits in
+  // Moving on to the pn length which is part of the protected bits
+  let pn_len = LowParse.BitFields.get_bitfield bits 0 2 in
+  assert (0 <= pn_len /\ pn_len <= 3);
+  let pnmask = QUIC.Spec.Lemmas.and_inplace (Seq.slice mask 1 (pn_len + 2)) (QUIC.Spec.pn_sizemask_naive pn_len) 0 in
+  assert (let l = Seq.length pnmask in 1 <= l /\ l <= 4);
+  // Classify, because HACL* specs require secret integers.
+  let pnmask = Seq.init (Seq.length pnmask) (fun i -> Lib.IntTypes.u8 (UInt8.v (Seq.index pnmask i))) in
+  let cipher = Seq.slice padded_cipher 0 (pn_len + 1) in
+  assert (Seq.length cipher == Seq.length pnmask /\ Seq.length cipher == pn_len + 1);
+  let pn = QUIC.Spec.Lemmas.pointwise_op (Lib.IntTypes.(logxor #U8 #SEC)) cipher pnmask 0 in
+  (| pn_len + 1, PNEPlainPkg?.mk u.plain j (pn_len + 1) pn bits |)
+
+val decrypt:
   (#j:id) ->
   (#u:info j) ->
   (st:pne_state u) ->
   (cp:pne_cipherpad) ->
   (s:sample) ->
   ST (option(l:pne_plain_length & pne_plain u l))
-  (requires fun h0 -> True)
+  (requires fun h0 ->
+    invariant st h0)
   (ensures fun h0 r h1 ->
     modifies_none h0 h1 /\ (
     if is_safe j then
@@ -230,21 +275,5 @@ val decrypt :
           (l = l' /\ c' `pne_bits_eq` clip_cipherpad cp l))
     else
       let cipher, encrypted_bits = cp in
-      // This mimics the specification of header_decrypt_aux starting after:
-      // let sample = ...
-      let mask = QUIC.Spec.block_of_sample u.calg (key st h0) s in
-      // Decrypting protected bits
-      let mask_bits: protected_bits = LowParse.BitFields.get_bitfield (UInt8.v (Seq.index mask 0)) 0 5 in
-      let bits = mask_bits `FStar.UInt.logxor` encrypted_bits in
-      // Moving on to the pn length which is part of the protected bits
-      let pn_len = LowParse.BitFields.get_bitfield bits 0 2 in
-      assert (0 <= pn_len /\ pn_len <= 3);
-      let pnmask = QUIC.Spec.Lemmas.and_inplace (Seq.slice mask 1 (pn_len + 2)) (QUIC.Spec.pn_sizemask_naive pn_len) 0 in
-      assert (let l = Seq.length pnmask in 1 <= l /\ l <= 4);
-      // Classify, because HACL* specs require secret integers.
-      let pnmask = Seq.init (Seq.length pnmask) (fun i -> Lib.IntTypes.u8 (UInt8.v (Seq.index pnmask i))) in
-      let cipher = Seq.slice cipher 0 (pn_len + 1) in
-      assert (Seq.length cipher == Seq.length pnmask /\ Seq.length cipher == pn_len + 1);
-      let pn = QUIC.Spec.Lemmas.pointwise_op (Lib.IntTypes.(logxor #U8 #SEC)) cipher pnmask 0 in
-      r == Some (| pn_len + 1, PNEPlainPkg?.mk u.plain j (pn_len + 1) pn bits |)
+      r == Some (decrypt_spec u.calg cipher encrypted_bits (key st h0) s)
   ))
