src/Model.PNE.fst
@@ -1,0 +1,102 @@
+module Model.PNE
+
+module B = LowStar.Buffer
+module HS = FStar.HyperStack
+module I = Model.Indexing
+module U32 = FStar.UInt32
+module U128 = FStar.UInt128
+module Spec = Spec.Agile.Cipher
+
+module ST = FStar.HyperStack.ST
+
+#set-options "--fuel 0 --ifuel 0"
+
+open FStar.HyperStack
+open Mem
+open Model.Helpers
+open LowStar.BufferOps
+
+let clip_cipherpad cp l =
+  let cipher, bits = cp in
+  Seq.slice cipher 0 l, bits
+
+let log (#i: id) (u: info i): Type0 =
+  Seq.seq (entry #i u)
+
+let model_state j =
+  u:info j & B.pointer (log #j u)
+
+let unsafe_state j =
+  // JP: I don't understand why we have to go through model.indexing here when
+  // the algorithm is readily available in the info
+  info j & Spec.key (I.pne_id_ginfo j)
+
+// JP: why is this type parameterized over the info?
+let pne_state #j u =
+  if is_safe j then
+    s:model_state j { dfst s == u }
+  else
+    s:unsafe_state j { fst s == u }
+
+let table #j #u st h =
+  let (| u, p |) = st <: model_state j in
+  B.deref h p
+
+let key #j #u st h =
+  snd (st <: unsafe_state j)
+
+let footprint #i #u w =
+  if is_safe i then
+    B.loc_addr_of_buffer (dsnd (w <: model_state i))
+  else
+    B.loc_none
+
+let invariant #i #u st h =
+  if is_safe i then
+    B.live h (dsnd (st <: model_state i))
+  else
+    True
+
+let frame_invariant #_ #_ _ _ _ _ =
+  ()
+
+let frame_table #_ #_ _ _ _ _ =
+  ()
+
+let create j u =
+  if is_safe j then
+    let l: log #j u = Seq.empty #(entry #j u) in
+    ((| u, B.malloc q_pne_region l 1ul |) <: model_state j)
+  else
+    (u, random (Spec.key_length u.calg)) <: unsafe_state j
+
+let random_bits (): protected_bits =
+  LowParse.BitFields.get_bitfield #8 (UInt8.v (Lib.RawIntTypes.u8_to_UInt8 (Seq.index (random 1) 0))) 0 5
+
+let encrypt #j #u st #l n s pn_length =
+  let h0 = ST.get () in
+  if is_safe j then
+    let (| u, p |) = st <: model_state j in
+    let log = !*p in
+    assert (log == table st h0);
+    let cipher: pne_cipher l = random l, random_bits () in
+    p *= Seq.snoc log (Entry s #l n cipher);
+    cipher
+  else
+    let open QUIC.Spec.Lemmas in
+    let pn, bits = PNEPlainPkg?.repr u.plain j l n in
+    let k = snd (st <: unsafe_state j) in
+    let alg = (fst (st <: unsafe_state j)).calg in
+    encrypt_spec alg l pn bits s k pn_length
+
+let decrypt #j #u st cp s =
+  if is_safe j then
+    let (| info, p |) = st <: model_state j in
+    let log = !*p in
+    match Seq.find_l (sample_filter u s) log with
+    | None -> None
+    | Some (Entry _ #l' n' c') ->
+        admit ()
+  else
+    let info, k = st <: unsafe_state j in
+    Some (decrypt_spec info.calg (fst cp) (snd cp) k s)
